	\begin{figure}[H]
		\centering
 \includegraphics[width=0.75\columnwidth]{chapters/11/10/1/2/figs/triangle.png}
		\caption{$a = 2$.}
		\label{fig:11/10/1/2}
  	\end{figure}
	Let the base be $BC$.  From the given information, 
\begin{align}
	\vec{B} = a\vec{e}_2,
	\vec{C} = -a\vec{e}_2
\end{align}
Since $\vec{A}$ lies on the $x$-axis, 
\begin{align}
	\vec{A} = k\vec{e}_1
\end{align}
and 
\begin{align}
	\norm{\vec{A}-\vec{C}}^2 &= \brak{2a}^2
	\\
	\implies \norm{\vec{A}}^2+\norm{\vec{C}}^2 - 2 \vec{A}^{\top}\vec{C} &= 4a^2
	\\
	\implies k^2 +a^2 &= 4a^2
\end{align}
yielding
\begin{align}
 k = \pm a\sqrt{3}
\end{align}
Thus, 
\begin{align}
	\vec{A} = \pm \sqrt{3}a\vec{e}_1
\end{align}
		See \figref{fig:11/10/1/2}.

